src/main/scala/qrhl/tactic/RuleTac.scala
@@ -1,0 +1,32 @@
+package qrhl.tactic
+
+import info.hupel.isabelle.ml.Expr
+import info.hupel.isabelle.pure
+import org.log4s
+import qrhl._
+import qrhl.logic.Expression
+import qrhl.toplevel.Parser
+
+import scala.collection.immutable.Nil
+
+case class RuleTac(rule:String) extends Tactic {
+  override def apply(state: State, goal: Subgoal): List[Subgoal] =
+    goal match {
+      case _: QRHLSubgoal => throw UserException("Expected an ambient logic subgoal")
+      case AmbientSubgoal(expr) =>
+        state.isabelle match {
+          case Some(isa) =>
+            val ml = Expr.uncheckedLiteral[String => pure.Term => pure.Context => List[pure.Term]]("QRHL.applyRule")
+            val goalsExpr = ml(rule)(implicitly)   (expr.isabelleTerm)(implicitly)   (isa.contextExpr)
+            val goals = state.isabelle.get.runExpr(goalsExpr)
+            for (t <- goals) yield AmbientSubgoal(Expression(isa,state.boolT,t))
+          case None => throw UserException(Parser.noIsabelleError)
+        }
+    }
+
+  override def toString: String = "rule "+rule
+}
+
+object RuleTac {
+  private val logger = log4s.getLogger
+}
