src/test/scala/qrhl/tactic/RuleTacTest.scala
@@ -1,0 +1,28 @@
+package qrhl.tactic
+
+import org.scalatest.{FlatSpec, FunSuite}
+import qrhl.toplevel.{Toplevel, ToplevelTest}
+
+class RuleTacTest extends FlatSpec {
+  def toplevel(): Toplevel = {
+    val tl = ToplevelTest.makeToplevel()
+    tl.run(
+      """ambient var a : nat.
+        |ambient var b : nat.
+        |ambient var c : nat.
+        |ambient var d : nat.
+      """.stripMargin)
+    tl
+  }
+
+  "rule tactic" should "produce new subgoals" in {
+    val tl = toplevel()
+    tl.execCmd("lemma test: a+b <= c+d")
+    val state2 = tl.state.applyTactic(RuleTac("add_le_mono"))
+    print("New goals: ",state2.goal)
+    state2.goal.foreach(_.checkWelltyped())
+    assert(state2.goal.length==2)
+    // TODO: check the goals themselves?
+  }
+
+}
